divRem and lt

SP1Operations/IsZeroOperation.lean
@@ -1,30 +1,29 @@
--- import SP1Foundations
+import SP1Foundations
 
--- structure IsZeroOperation where
---   /-- The inverse of the input. -/
---   inverse : U16
---   /-- Result indicating whether the input is 0. This equals `inverse * input == \ 0`. -/
---   result  : U1
+structure IsZeroOperation where
+  inverse : Fin BB
+  result : Fin BB
 
--- namespace IsZeroOperation
+namespace IsZeroOperation
 
--- def spec (cols : IsZeroOperation)
---     (a : U16) (is_real : U1) : Prop :=
---   is_real = 1 → (a = 0 ↔ cols.result = 1)
+def constraints
+  (a : (Fin BB))
+  (cols : IsZeroOperation)
+  (is_real : (Fin BB))
+  : SP1ConstraintList :=
+  let E0 : Fin BB := cols.inverse * a
+  let E1 : Fin BB := 1 - E0
+  let E2 : Fin BB := E1 - cols.result
+  let E3 : Fin BB := is_real * E2
+  let E4 : Fin BB := cols.result - 1
+  let E5 : Fin BB := cols.result * E4
+  let E6 : Fin BB := is_real * E5
+  let E7 : Fin BB := cols.result * a
+  let E8 : Fin BB := is_real * E7
+  [
+    (.assertZero E3),
+    (.assertZero E6),
+    (.assertZero E8),
+  ]
 
--- def constraints (cols : IsZeroOperation)
---     (a : U16) (is_real : U1) : SP1ConstraintList :=
---   [
---     .assertZero (is_real.val * ((1 - (cols.inverse.val * a.val)) - cols.result.val)),
---     .assertZero (is_real.val * (cols.result.val * (cols.result.val - 1))),
---     .assertZero (is_real.val * (cols.result.val * (cols.result.val - 1))),
---     .assertZero (is_real.val * (cols.result.val * a.val))
---   ]
-
--- theorem correct (cols : IsZeroOperation)
---     (a : U16) (is_real : U1) :
---     (cols.constraints a is_real).allHold → cols.spec a is_real := by
---   simp [constraints, spec, sub_eq_zero]
---   aesop
-
--- end IsZeroOperation
+end IsZeroOperation
