SP1Chips.lean
@@ -1,4 +1,6 @@
 import SP1Chips.AddChip
 import SP1Chips.BitwiseChip
+import SP1Chips.DivRem
 import SP1Chips.JalChip
+import SP1Chips.LtChip
 import SP1Chips.MulChip
